aarch64 refine: SMC caps
Similarly to AInvs in the previous commit, introduce an arch_capBadge
interface with corresponding lemmas since SMC caps have badges and use
the general badge mechanisms.

The previous assumption that arch caps do not have badges also comes out
in the is_arch_update' predicate which now needs to explicitly demand
that the cap badge is None. This actually simplifies some proofs in the
architecture dependent part, but needs minor updates in Orphanage.

Also move up the definition of arch_cap'_fun_lift and introduce an
abbreviation arch_cap'_pred that can be used to lift arch cap predicates
to all caps (returning False on generic caps).

Signed-off-by: Gerwin Klein <gerwin.klein@proofcraft.systems>

proof/refine/CSpace_I.thy
@@ -17,6 +17,7 @@ arch_requalify_facts (H)
 
 locale CSpace_I =
   fixes arch_capMasterCap :: "arch_capability \<Rightarrow> arch_capability"
+  fixes arch_capBadge :: "arch_capability \<Rightarrow> machine_word option"
   assumes isPhysicalCap[simp]:
     "\<And>cap. isPhysicalCap cap = (capClass cap = PhysicalClass)"
   assumes isArchFrameCap_non_arch:
@@ -545,9 +546,12 @@ lemma isDomainCap[simp]:
   "isDomainCap cap = (cap = DomainCap)"
   by (rule gen_isCap_simps)
 
+context CSpace_I begin
+
 definition capBadge :: "capability \<Rightarrow> machine_word option" where
   "capBadge cap \<equiv> if isEndpointCap cap then Some (capEPBadge cap)
                   else if isNotificationCap cap then Some (capNtfnBadge cap)
+                  else if isArchObjectCap cap then arch_capBadge (capCap cap)
                   else None"
 
 lemma capBadge_simps[simp]:
@@ -559,13 +563,11 @@ lemma capBadge_simps[simp]:
   "capBadge (CNodeCap ref bits gd gs)          = None"
   "capBadge (ThreadCap ref)                    = None"
   "capBadge (Zombie ref b n)                   = None"
-  "capBadge (ArchObjectCap cap)                = None"
+  "capBadge (ArchObjectCap cap)                = arch_capBadge cap"
   "capBadge (IRQControlCap)                    = None"
   "capBadge (IRQHandlerCap irq)                = None"
   "capBadge (ReplyCap tcb master g)            = None"
   by (simp add: capBadge_def gen_isCap_defs)+
-
-context CSpace_I begin
 
 definition capMasterCap :: "capability \<Rightarrow> capability" where
   "capMasterCap cap \<equiv> case cap of
